\input{notes.tex}


\iftoggle{dualscreen}{\setbeameroption{show notes on second screen=right}}{}

\settoggle{covered}{true}
\begin{document}
\section{Lecture 17}
\subsection{Laplace Transforms Practice}

\slide[Laplace Inversion Tactics]{\small
\enum{
\item Function has denominator that can factor.
\subitem{factor and use partial fraction decomposition}
\[\frac{1}{(s+a)s}=\frac{1}{as}-\frac{1}{a(s+a)} \quad \underrightarrow{\mathcal{L}^{-1}}\quad  \frac{1}{a}-\frac{1}{a}e^{-at}\]
\item Denominator has something with $(s-a)^n$ but numerator has $s$ appearing in it, not $s-a$. \vfill
\subitem{Split numerator by adding/subtracting so that all appearances of $s$ are in the form $s-a$ \item use First Shift Theorem to invert}\[\frac{s}{(s-a)^n}=\frac{s-a}{(s-a)^n}+\frac{a}{(s-a)^n} \quad \underrightarrow{\mathcal{L}^{-1}}\quad \frac{e^{at}t^{n-2}}{(n-2)!}+\frac{a}{(n-1)!}e^{at}t^{n-1}\]\vfill
\item Numerator has incorrect constant $A$ for inversion. \subitem{Mulitply by $\frac{\omega}{\omega}$ and swap $\omega$ with $A$ :\[\frac{\omega}{\omega}\frac{A}{\omega^2+s^2}=\frac{A}{\omega}\frac{\omega}{\omega^2+s^2}\quad \underrightarrow{\mathcal{L}^{-1}}\quad   \frac{A}{\omega}\sin(\omega t) \] }
}
}

\slide{\ex{$y\pp+2y\p+5y=0$, \quad $y(0)=y_0$, $y\p(0)=v_0$}
\student{
\algn{s^2Y(s)-&sy_0-v_0+2sY(s)-2y_0+5Y(s)=0\\
Y(s)&=\frac{sy_0+v_0+2y_0}{s^2+2s+5}=\frac{sy_0+v_0+2y_0}{\underbrace{s^2+2s+1}_{(s+1)^2}\underbrace{-1+5}_{2^2}}\\
&=\frac{sy_0+v_0+2y_0}{(s+1)^2+2^2 } =\frac{sy_0}{(s+1)^2+2^2 } + \frac{v_0+2y_0}{(s+1)^2+2^2 }\\
&=y_0 \lap{e^{-t}\underbrace{\lapinv{\frac{s}{s+2^2}}}_{\cos(2t)}}+(v_0+y_0 )\lap{e^{-t} \underbrace{\lapinv{\frac{1}{s^2+2^2}}}_{\frac12 \sin(2t)}}\\\\
y(t)&=y_0e^{-t}\cos(2t)+\frac{v_0+y_0}{2}e^{-t}\sin(2t)} 
}
}%end slide

\slide{\ex{$y\pp+12y\p+36y=0$, \quad $y(0)=y_0$, $y\p(0)=v_0$}

\student{
\algn{s^2Y(s)-&sy_0-v_0+12sY(s)-12y_0+36Y(s)=0\\
Y(s)&=\frac{sy_0+v_0+12y_0}{s^2+12s+36}=\frac{sy_0+v_0+12y_0}{(s+6)^2}\\
&=\frac{y_0\cancel{(s+6)}}{(s+6)^{\cancel{2}}}+\frac{v_0+12y_0-6y_0}{(s+6)^2}\\
&=y_0\underbrace{\frac{1}{s+6}}_{\lap{e^{-6t}}}+(v_0+6y_0) \frac{1}{(s+6)^2}\\
&=y_0\lap{e^{-6t}}  +(v_0+6y_0) \lap{e^{-6t} \lapinv{\frac{1}{s^2}}}\\\\
y(t)&=y_0e^{-6t}+(v_0+6y_0)e^{-6t}t} 
}

}%end slide

\slide{\ex{$y\p+6y=u_1(t)\student{=\begin{cases}
0 & t<1\\
1 & t\geq1
\end{cases}}$}
\student{\twomini[.55]{.6}{.3}{\algn{ sY-&y_0+6Y=\frac{e^{-s}}{s}\\
Y&=\frac{\frac{e^{-s}}{s}+y_0}{s+6}=\frac{e^{-s}}{s(s+6)}+\frac{y_0}{s+6}\\
Y(s)&=\frac{1}{6}\frac{e^{-s}}{s}-\frac{1}{6}\frac{e^{-s}}{s+6}+\frac{y_0}{s+6}\\
& \downarrow \mathcal{L}^{-1}\\
y(t)&=\frac16 u(t-1)-\frac16 e^{-6(t-1)} u(t-1)+y_0e^{-6t}
}\vfill}{$\frac{1}{s(s+6)}=\frac{A}{s}+\frac{B}{s+6}$\\~\\$\Rightarrow 1=A(s+6)+Bs $\\~\\$\Rightarrow \arr{l}{1=6A\\0=A+B}$ \\~\\$\Rightarrow \arr{l}{A=\frac16\\B=-\frac16}$ \vfill}}
\tikzplot[
\student{\xcoord{3}{1} \ycoord{1.25}{\frac16}}
]{.1}{10}{.1}{1.5}{t}{y(t)}{
\student{
\draw[domain=0:2, thick, samples=100] plot ({\x*1.5}, {.8*exp(-\x)});
\draw[domain=2:10, thick, samples=100] plot ({\x*1.5}, {.8*exp(-\x)+(1-exp(-(\x-2)))*1.25});
\draw[domain=0:10, thick, dashed, samples=100] plot ({\x*1.5}, {1.25});
}}
}



\slide{\ex{$y\pp+2y\p+5y=u_5(t)-u_{15}(t)$, \quad $y(0)=y_0$, $y\p(0)=v_0$}
\student{
\algn{s^2Y(s)-&sy_0-v_0+2sY(s)-2y_0+5Y(s)=\frac{e^{-5s}}{s} - \frac{e^{-15s}}{s}\\
Y(s)&= \frac{  \paren{\frac{e^{-s}}{s} - \frac{e^{-2s}}{s}} + sy_0+v_0+2y_0}{s^2+2s+5}\\
&=  \paren{ e^{-5s} - e^{-15s}}  \underbrace{\frac{ 1}{s(s^2+2s+5)}}_{F(s)}+   \underbrace{\frac{ sy_0 +v_0 +2y_0}{s^2+2s+5}}_{\text{homogeneous part}}\\\\
y(t)&=u_5(t)\left[ \lapinv{F(s)} \right]_{t=t-5}\\
&\phantom{=} - u_{15}(t)\left[ \lapinv{F(s)} \right]_{t=t-15}\\
&\phantom{=} + y_0e^{-t}\cos(2t)+\frac{v_0+y_0}{2}e^{-t}\sin(2t)
}
}
}%end slide

\settoggle{covered}{false}
\slide{$\lapinv{\frac{1}{s(s^2+2s+5)}}=\;???$ 

\student{
\algn{F(s)=\frac{1}{s(s^2+2s+5)} & = \frac{A}{s} +\frac{Bs+C}{s^2+2s+5}\\
1&=As^2+2As+5A + Bs^2+Cs\\
\text{constant terms: } 1&= 5A \qquad \Rightarrow A=\frac15 \\
\text{$s$ terms: } 0 &= 2A+C   \qquad \Rightarrow C=-2A=-\frac25\\
\text{$s^2$ terms: } 0 &=	A+B  \qquad \Rightarrow B=-A=-\frac15\\
F(s) &= \frac{1}{5s} - \frac15 \frac{s+2}{(s+1)^2+2^2}\\
&=  \frac{1}{5s} -  \frac15 \paren{\frac{s+1}{(s+1)^2+2^2}  - \frac{1}{(s+1)^2+2^2}}  \\
f(t) &= \frac15 \paren{1-e^{-t}\paren{cos(2t) -\frac12 \sin(2t)}}}
}
}

\slide{\vspace{-2em}
\algn{y(t)&=u_5(t)\frac15 \paren{1-e^{-(t-5)}\paren{cos(2(t-5)) -\frac12 \sin(2(t-5))}}\\
&\phantom{=} - u_{15}(t)\frac15 \paren{1-e^{-(t-15)}\paren{cos(2(t-15)) -\frac12 \sin(2(t-15))}}\\\
&\phantom{=} + y_0e^{-t}\cos(2t)+\frac{v_0+y_0}{2}e^{-t}\sin(2t)}

\vspace{1em}
$y_0=0.1, v_0=0$
\centerline{\includegraphics[width=8.5cm]{images/Heaviside_jiggle.pdf}}
}

\slide{\ex{$y\pp+y\p=1$, $y(0)=y_0$, $y\p(0)=v_0$}
\student{\vspace{-.5em}
\algn{s^2Y(s)-&sy_0-v_0+sY(s)-y_0=\frac1s\\
(s^2+s)Y&=sy_0+y_0+v_0+\frac1s\\
Y(s)&=\frac{\cancel{s}y_0}{\cancel{s}(s+1)}+\frac{y_0+v_0}{s(s+1)}+\frac{1}{s^2(s+1)}}\vspace{-1.5em}
\algn{\frac{1}{s(s+1)}&=\frac{A}{s}+\frac{B}{s+1}&\arr{r}{1=A(s+1)+Bs\\A=1, B=-1}\\
&=\frac1s-\frac{1}{s+1}\\
\frac{1}{s^2(s+1)}&=\frac{A}{s^2}+\frac{B}{s}+\frac{C}{s+1}&\arr{r}{1=A(s+1)+Bs(s+1)+Cs^2\\\uline{s=0:}\;A=1,\quad  \uline{s=-1:}\;C=1}\\
&=\frac{1}{s^2}-\frac{1}{s}+\frac{1}{s+1}&\uline{s=1:}\; 2+2B+\cancel{1}=\cancel{1}}\vspace{-1.5em}
\algn{Y(s)&=\cancel{\frac{y_0}{s+1}}+\frac{y_0+v_0}{s}-\frac{\cancel{y_0}+v_0}{s+1}+\frac{1}{s^2}-\frac{1}{s}+\frac{1}{s+1}&B=-1}
}
}%end slide

\slide{continuing $\dots Y(s)=\frac{y_0+v_0-1}{s}+\frac{1-v_0}{s+1}+\frac{1}{s^2}$
\student{\algn{y(t)&=y_0+v_0+1+(1-v_0)e^{-t}+t\\
&=\underbrace{c_1+c_2e^{-t}}_{y_h}+\underbrace{t}_{y_p}\intertext{\uline{M.U.C.}}
y\pp+y\p&=1\intertext{homogeneous problem}
&r^2+r=0\Rightarrow r(r+1)=0 &\Rightarrow y_h=c_1+c_2e^{-t} \intertext{RHS in nullspace of operator}
y_p=Bt \dots}
put it all together and then solve for $c_1$ and $c_2\dots$
}

}%end slide


\end{document}
