\input{notes.tex}


\iftoggle{dualscreen}{\setbeameroption{show notes on second screen=right}}{}


\begin{document}

\section{Lecture 7}
\subsection{Introduction}


\slide[Recall: Constant Coefficients 2$^{nd}$ Order Homogeneous IVP]{
\[ay\pp +by\p +cy= h(t) =0 \qquad \carray {y(0)=y_0\\ y\p (0)=v_0}\]
\ex{Spring-dashpot with no external forcing}
\[y_h(t)=c_1y_1(t)+c_2y_2(t) \qquad -\qquad  \text{three major cases}\]
What about for the inhomogeneous case ($h(t)\neq0$) ?
\vfill
General solution:
\[y_g = y_p +y_h\]
\vfill\student{
Recall, $y_p$ has no arbitrary coefficients.
\vfill
How can we find $y_p$?}

}

\slide[$ay\pp +by\p +cy = h(t) \neq 0 $]{
Two major cases:
\student{
\enum{
\item $c=0$\vfill
Define $v(t)=y\p$
\[av\p+bv=h(t)\]
Solve by method of integrating factors
\item $c\neq0$\vfill
\centerline{Method of Undetermined Coefficients}
}
}
}

\slide[$ay\pp +by\p +cy = h(t) \neq 0 $]{
$c\neq0$ \hfill -\hfill Method of Undetermined Coefficients\vfill
\student{
Basic idea
\[y_g = y_p +y_h\]
We know how to find $y_h$\subitem{ it makes the LHS=0}\vfill

When we plug $y_p$ into the LHS, it must equal $h(t)$.
\subitem{$y_p$ + its derivatives = $h(t)$}\vfill

Idea: differentiate $h(t)$ a bunch and see what kind of funtion $y_p$ could be.

}
}

\slide[Find all the functional forms obtained by differentiation]{
$h(t)=t^2$
\student{\[\{  t^2, t, \text{constant}\} \qquad \text{finite set}\]}
\vfill
$h(t)=\cos(3t)$
\student{\[\left\{ \sin(3t), \cos(3t)\right\} \qquad \text{finite set} \]}
\vfill
$h(t)=\ln(t)$
\student{\[\left\{ \ln(t), \frac1t, \frac{1}{t^2}, \frac{1}{t^3}, \dots \right\} \qquad \text{infinite set}\]}
}

\slide[Find the particular solution to $3y\pp+2y\p+y=t^2$]{\vspace{-0.75em}
Hint: guess $y_p=A+Bt+Ct^2$
\student{\algn{
y_p\p&=B+2Ct & y_p\pp&=2C\intertext{plug into ODE}
6C+&2(B+2Ct)+A+Bt+Ct^2=t^2\\
&Ct^2 + (4C+B)t+(A+2B+6C)=t^2
}
We need this to be true for all $t$. Equate the coefficients in front of the different time-dependent functions.
\algn{\uline{t^2}: C &= 1 & \uline{t}:  (4C+B)&=0\\
\uline{\text{constant}}: A+2B+6C&=0 &4+B&=0& B=-4\\
A-8+6&=0&\Rightarrow A=2}\vfill
\[y_p=2-4t+t^2\]
}

}

\slide[Find the particular solution to $y\pp+3y=24e^{3t}$]{\vspace{-0.75em}
\student{
Guess $y_p(t)=Ae^{3t}$
\algn{
y_p\p&=3Ae^{3t}& y_p\pp&=9Ae^{3t}\intertext{plug into ODE}
9Ae^{3t}+3Ae^{3t}&=24e^{3t}\\
12Ae^{3t}&=24e^{3t}
}
We need this to be true for all $t$. Equate the coefficients in front of the different time-dependent functions.
\algn{\uline{e^{3t}}: 12A &= 24 & A&=2\\\\
y_p(t)&=2e^{3t}
}
}
}

\slide[$ay\pp +by\p +cy = h(t) \neq 0 $]{
Will that approach always work?\vfill
\student{
Yes, if the function $h(t)$ has a finite family of derivative functional forms.
\vfill
\ex{$e^{t}, t^8, te^t, \cos(t), \sin(t), \dots$}
\vfill
No, if it has infinitely many derivatives...\vfill
\ex{$\ln(t), t^{-1}, t^{-2},\dots$}

}}

\subsection{Method of Undetermined Coefficients}
\slide[\begin{minipage}{.5\textwidth}Method of Undetermined\\ Coefficients:\end{minipage}\hfill\begin{minipage}{.34\textwidth}$\rarray{ay\pp+by\p+cy=h(t)\\y(t)=y_p(t)+y_h(t)}$\end{minipage}]{

\small
\vfill
\begin{table}\setlength\extrarowheight{5pt}
\begin{tabular}{|c|c|}
\hline 
Form of function $h(t)$ & Geuss for $y_{p}\left(t\right)$\tabularnewline
\hline 
\hline 
$\sum_{j=0}^{N}B_{j}t^{j}$ & $\sum_{j=0}^{N}A_{j}t^{j}$\tabularnewline
\hline 
$e^{\lambda t}$ & $Ae^{\lambda t}$\tabularnewline
\hline 
$\sin \omega t$ or $\cos  \omega t$ & $A\sin \omega t+B\cos \omega t$\tabularnewline
\hline 
$e^{\lambda t}\sin \omega t$ or $e^{\lambda t}\cos \omega t$ & $e^{\lambda t}A\sin \omega t+e^{ \lambda t}B\cos \omega t$\tabularnewline
\hline 
Additive combinations of above & Additive combinations of above\tabularnewline
\hline 
Multiplicative combinations of above & Multiplicative combinations of above\tabularnewline
\hline 
Part of the homogeneous solution {\tiny Note}\footnotemark& $Ath(t) \text{ or } At^2h(t)$ \text{ or } \dots \tabularnewline
\hline 
Anything else & You are out of luck\tabularnewline
\hline 
\end{tabular}
\end{table}\vfill

\footnotetext[1]{Note: This corresponds to resonance. }
\footnotetext[2]{Note: $b_j$ , $c_j$ , $b$, $c$, $A$, and $B$ are all constants in the above table}


}

\slide{Find the particular solution to $y\pp -6y\p+\frac{25}{4}y =3te^{2t}$\vfill
\student{
guess $y_p = Ae^{2t}+Bte^{2t}$
\algn{y_p\p&=2Ae^{2t}+Be^{2t} +2Bte^{2t} &y_p\pp&=2(2A+B)e^{2t} + 2Be^{2t}+4Bte^{2t}\\
&=(2A+B)e^{2t}+2Bte^{2t}&&=4(A+B)e^{2t} + 4 B t e^{2t}\intertext{plug into DE}
}\vspace{-3em}
\algn{4(A+B)e^{2t} + 4 B t e^{2t} - 6(2A+B)e^{2t}-12Bte^{2t} + \frac{25}{4}Ae^{2t}+\frac{25}{4}&Bte^{2t}&\\&=3te^{2t}}
\vspace{-2em}
\algn{
-\frac74Bte^{2t} -& \frac14\paren{7A+8B}e^{2t}=3te^{2t} \\
\uline{te^{2t}}:  -\frac74B&=3  & B&=-\frac{12}{7}\\
\uline{e^{2t}}:  7 A + 8 B &=0  & A&=\frac{8\cdot12}{7\cdot7}=\frac{96}{49}}\vfill
\[y_p =\frac{96}{49}e^{2t} -\frac{12}{7}te^{2t} \]
}
}

\slide{Solve the IVP $y\pp -3y\p -4y =3e^{2t}$ with $ y(0)=y\p(0)=1$
\student{
\[ y_g=y_p+c_1y_1+c_2y_2 \]
\algn{
y_{1,2}=e^{rt}\quad & \Rightarrow \quad (r^2-3r-4)=0\\
r_{1,2} &= \frac{3\pm\sqrt{9+16}}{2} =\frac{3\pm 5}{2} = 4,-1 \\\\
 y_g &= c_1 e^{4t} + c_2 e^{-t} -\frac12 e^{2t}\\
 y_g\p &= 4 c_1 e^{4t} - c_2 e^{-t} - e^{2t}\intertext{Initial Conditions:}
y(0)=1=c_1 + c_2 -\frac12\\
y\p(0)=1 = 4c_1-c_2-1
}

}
}
\slide{\vspace{-2em}\algn{y(0)=1=c_1 + c_2 -\frac12\\
y\p(0)=1 = 4c_1-c_2-1}
\student{\vspace{-2em}
\algn{\intertext{Add the two equations}
2&=5c_1-\frac32& 
\frac{7}{2} &= 5c_1 \\ c_1 &=  \frac{7}{10} \\
1&=\frac{7}{10} + c_2 -\frac{5}{10} &
1&=\frac{2}{10}+c_2\\
c_2&=\frac{8}{10}\\\\
y(t)&=\frac{7}{10}e^{4t} + \frac{8}{10}e^{-t} -\frac12e^{2t}
}
}
}
 



\end{document}