\input{notes.tex}


\iftoggle{dualscreen}{\setbeameroption{show notes on second screen=right}}{}
\usetikzlibrary{arrows}

\begin{document}
\section{Lecture 13}
\subsection{Theory}

\slide[Recall:]{
 \[\dd{}{t}\vec{x} = \mathbf{A}(t) \vec{x} \qquad \text{with } \mathbf{A} \text{ an } n\times n \text{ matrix} \]
\vfill
We can find $n$ solutions $\vec{x}(t)=e^{\lambda t}\vec{v}$ by finding the eigenvalues, $\lambda$, and eigenvectors, $\vec{v}$, of the matrix $\mathbf{A}$.\vfill
\vfill
i.e., solving
   \[\det(\mathbf{A} - \lambda \mathbf{I}) = 0\quad\text{and}\quad (\mathbf{A} - \lambda \mathbf{I})\vec{v}= 0\]
}

\slide[Homogeneous Problem and Superposition]{\vspace{-1em}
Suppose $\vec{x}_1(t), \;\vec{x}_2(t),\;\dots, \;\vec{x}_n(t)$ all solve the homogeneous problem \[\dd{}{t}\vec{x} = \mathbf{A}(t) \vec{x} \]\vfill
Then \[\vec{x}(t) = c_1\vec{x}_1(t)+c_2\vec{x}_2(t)+\dots+c_n\vec{x}_n(t)\]
also solves the same homogeneous problem.
\vfill
\student{
\algn{\dd{}{t}\vec{x} &= \sum_{i=1}^nc_i\dd{}{t}\vec{x}_i= \sum_{i=1}^nc_i \mathbf{A}(t) \vec{x}_i \\& =  \mathbf{A}(t)  \sum_{i=1}^nc_i\vec{x}_i \\
&=\mathbf{A}(t)\vec{x}(t)}
So, the $\vec{x}(t)$ above is the general solution to the homogeneous problem.
}
}
\subsection{Examples}
\slide[Find the general solution to \hfill \small $\larray{ \dd{x}{t} = -3x - 2y \\ \dd{y}{t} = -2x - 6y}$]{\student{\vspace{-3em}
\algn{\vec{x}(t)&=c_1\vec{x}_1(t) + c_2 \vec{x}_2(t)\\
&=c_1\underbrace{\underbrace{\mat{c}{-2\\1}}_{\text{eigenvector}}e^{-2t}}_{\text{eigensolution}} + c_2 \mat{c}{1\\2}e^{-7t}
}
Notes:
\itmz{\item The two eigenvectors are linearly independent
\subitem{$\Rightarrow$ The two eigensolutions/eigenmodes are linearly independent}
\item The solution has components along the two eigenvectors/eigendirection
\item The component along the second direction decays the fastest.
\item $c_1$ and $c_2$ are determined from initial conditions
}
}
}


\slide[Find the  solution to \hfill \small $\larray{ \dd{x}{t} = -3x - 2y \\ \dd{y}{t} = -2x - 6y}$ with $\larray{x(0)=5\\\\ y(0)=4}$]{\student{\vspace{-2em}
\algn{\ucover{\vec{x}(t)}&\ucover{=c_1\mat{c}{-2\\1}e^{-2t} + c_2 \mat{c}{1\\2}e^{-7t}}\\
\vec{x}(0)&=c_1\mat{c}{-2\\1} + c_2 \mat{c}{1\\2}  = \mat{c}{5\\4}\\
&\mat{cc|c}{-2c_1 & c_2 & 5\\c_1 &2c_2&4} \intertext{$2R_2+R_1\rightarrow R_1$ }
&\mat{cc|c}{0 & 5c_2 & 13\\c_1 &2c_2&4} 
 \intertext{$-\frac25R_1+R_2\rightarrow R_2$ }
&\mat{cc|c}{0 & 5c_2 & 13\\c_1 &0&-\frac{6}{5}}&\larray{c_1=-\frac65\\c_2=\frac{13}{5}} 
}
}
}

\slide[Initial Conditions and Eigenvectors]{
For first order systems of the form $\dd{}{t}\vec{x}=\mathbf{A}\vec{x}$, we have a general solution
 \[\vec{x}(t) = c_1\vec{x}_1(t)+c_2\vec{x}_2(t)+\dots+c_n\vec{x}_n(t),\] 
where with real and distinct eigenvalue of $\mathbf{A}$, we have: $\vec{x}_i(t)=e^{\lambda_i t}\vec{v}_i$
\student{
\enum{\vfill
\item The arbitrary coefficients $c_i$ come from decomposing the initial condition $\vec{x}(0)$ onto the basis of eigenvectors $\{\vec{v}_i\}$.\vfill
\item This decomposes the solution into $n$ different "eigenmodes".\vfill\subitem{$c_i$ is the initial "amplitude" of the $i^{th}$ eigenmode}\vfill
\item Each eigenmode grows ($\lambda_i>0$) or shrinks ($\lambda_i<0$) over time.
}
}
}

\slide[Find the general solution to \hfill \small $\larray{ \dd{x}{t} = - 2y \\ \dd{y}{t} = -2x - 3y}$]{\vspace{-1.5em}
\student{\algn{\dd{}{t} \mat{c}{x\\y}  &= \mat{cc}{0&-2\\-2&-3} \mat{c}{x\\y} \\ \det\left(  \mat{cc}{-\lambda&-2\\-2&-3-\lambda} \right) &= 0\\
-\lambda (-3-\lambda) - 4 &=0\\
\lambda^2 +3\lambda  - 4 &= 0\\
(\lambda-1)(\lambda+4) &=0\\
\lambda_{1,2} &=1, -4}
}
}

\slide[Find the general solution to \hfill \small $\larray{ \dd{x}{t} = - 2y \\ \dd{y}{t} = -2x - 3y}$]{\student{\vspace{-2em}
\algn{\uline{\lambda_1=1:} \quad &  \mat{cc|c}{0-1&-2 &0\\-2&-3-1&0} &&   \mat{cc|c}{-1&-2 &0\\-2&-1&0}
\intertext{row 2 and row 1 are linearly dependent: $R_2-2R_1\rightarrow R_2$}
& \mat{cc|c}{-1&-2 &0\\0&0&0} &-1x-2y&=0\\
&&x&=-2y\\
\vec{v}_1&=\mat{c}{-2\\1}&\vec{x}_1(t)&=\mat{c}{-2\\1}e^{t}
}
}
}

\slide[Find the general solution to \hfill \small $\larray{ \dd{x}{t} = - 2y \\ \dd{y}{t} = -2x - 3y}$]{\student{\vspace{-2em}
\algn{\uline{\lambda_2=-4:} \quad &    \mat{cc|c}{4&-2 &0\\-2&1&0}
\intertext{row 2 and row 1 are linearly dependent: $R_2+R_1/2\rightarrow R_2$}
& \mat{cc|c}{4&-2 &0\\0&0&0} &4x-2y&=0\\
&&2x&=y\\
\vec{v}_2&=\mat{c}{1\\2}&\vec{x}_2(t)&=\mat{c}{1\\2}e^{-4t}\\\\
\vec{x}(t) &= c_1\mat{c}{-2\\1}e^{t}+c_2\mat{c}{1\\2}e^{-4t}
}
}
}


\slide[Find the eigenvalues for the ODE:  \hfill \small $\larray{ \dd{x}{t} = -x + 2y \\ \dd{y}{t} = -2x - y}$]{\vspace{-1.5em}
\student{\algn{\mathbf{A}  &= \mat{cc}{-1&2\\-2&-1} \\
\det\left(  \mat{cc}{-1-\lambda&-2\\2&-1-\lambda} \right) &= 0\intertext{Characteristic equation}
 (-1-\lambda)^2 + 4 &=0\\
\lambda^2 +2\lambda  + 5 &= 0\\
\lambda_{1,2} &= \frac{-2\pm \sqrt{4-20}}{2} =\frac{-2\pm \sqrt{-16}}{2}\\
 \lambda_{1,2} &=  -1 \pm 2 i }
}
}

\slide[Complex conjugate eigenvalues pairs: $\lambda_{1,2}=r\pm i\omega $]{\vspace{-.5em}
\noindent Associated eigenvectors are also complex conjugates
\student{\[\vec{v}_{1,2}=\underbrace{\vec{a}}_{\text{real part}} \pm \underbrace{i\vec{b}}_{\text{imaginary part}}\]
\vfill
Proof:\vfill
Suppose $\vec{v}_{1}=\vec{a}+i\vec{b}$ with $\lambda_1=r+i \omega$
\algn{\mathbf{A} (\vec{a}+i\vec{b})  &= (r+i\omega) (\vec{a}+i\vec{b})\intertext{Take complex conjugate of both sides}
\mathbf{A} (\vec{a}-i\vec{b}) &=  (r-i\omega) (\vec{a}-i\vec{b})\\
\mathbf{A} \vec{v}_2 &=\lambda_2  \vec{v}_2  }
}
}

\slide[Find the eigenvectors for the ODE:  \hfill \small $\larray{ \dd{x}{t} = -x + 2y \\ \dd{y}{t} = -2x - y}$]{\vspace{-1.5em}
\student{\[ \lambda_{1,2} =  -1 \pm 2 i\]\vspace{-3em}
\algn{ \intertext{\uline{$\lambda_{1} =  -1 + 2 i$}} \mat{cc|c}{-1-(-1+2i)&2&0\\-2&-1-(-1+2i)&0} & \quad \rightarrow &\mat{cc|c}{-2i &2&0\\-2&-2i&0} \\
\intertext{$R_2-iR_1\rightarrow R_2$ and $\frac12 R_1 \rightarrow R_1$}
\mat{cc|c}{-i &1&0\\0&0&0} &&\rarray{ -i x + y = 0\\y=ix}\\\\
\vec{v}_1=\mat{c}{1\\i} = \mat{c}{1\\0}+i\mat{c}{0\\1}&  & \Rightarrow \vec{v}_2=\mat{c}{1\\-i} }
}
}

\slide[Find the general solution for the ODE:  \hfill \small $\larray{ \dd{x}{t} = -x + 2y \\ \dd{y}{t} = -2x - y}$]{\vspace{-1.5em}
\student{\[ \lambda_{1,2} =  -1 \pm 2 i \qquad \vec{v}_{1,2}=\mat{c}{1\\\pm i}\] 
\algn{\vec{x}(t) &= c_1e^{(-1+2i)t}\mat{c}{1\\ i} + c_2e^{(-1-2i)t}\mat{c}{1\\- i} \\\\
x(t)&=c_1 e^{(-1+2i)t} + c_2 e^{(-1-2i)t}\\
y(t)&=ic_1 e^{(-1+2i)t} - ic_2 e^{(-1-2i)t}
}\vfill
Can convert to purely real solution using Euler's identity (not covered).
}
}

\subsection{Summary}

\slide[General solution to the eigenproblem (2x2)]{
From linear algebra, we know that $\mathbf{A}\vec{v} = \lambda \vec{v}$ has a non-trivial solution $\vec{v}$ only if the determinant of the matrix $\mathbf{A}-\lambda \mathbf{I} $ is identically zero.
\vfill
That is, the constant $\lambda$ must satisfy the characteristic equation \[\det (\mathbf{A}-\lambda \mathbf{I})=0.\]\vfill
ex: $A=\mat{cc}{a&b\\c&d}$\student{$\det \left( \mat{cc}{a-\lambda &b\\c&d-\lambda} \right)=(a-\lambda)\cdot(d-\lambda)-bc=0$ \vfill
\algn{\underbrace{\lambda^2-(a+d)\lambda + ad - bc}_{\text{characterisitc poly.}} &=0 &\Rightarrow
\lambda = \frac{a+b\pm\sqrt{(a+d)^2-4(ad-bc)}}{2} }}
}

\slide[General solution to the eigenproblem (2x2)]{
From linear algebra, we know that $\mathbf{A}\vec{v} = \lambda \vec{v}$ has a non-trivial solution $\vec{v}$ only if the determinant of the matrix $\mathbf{A}-\lambda \mathbf{I} $ is identically zero.
\vfill
That is, the constant $\lambda$ must satisfy the characteristic equation \[\det (\mathbf{A}-\lambda \mathbf{I})=0.\]\vfill
\student{
Three possibilites
\enum{
\item $\mathbf{A}$ has 2 distinct real eigenvalues and eigenvectors\checkmark
\item The eigenvalues/vectors of  $\mathbf{A}$ occur as a complex conjugate pair \checkmark
\item One eigenvalue is repeated (not covered)
}}
}

\end{document}