\input{notes.tex}


\iftoggle{dualscreen}{\setbeameroption{show notes on second screen=right}}{}
\usetikzlibrary{arrows}

\begin{document}

\section{Lecture 18}

\subsection{Introduction}
\slide[Recall:]{
So far, we have always been rearranging $s$-domain functions to be \uline{sums} of easy to invert terms.
\vfill
\ex{$Y(s)=\frac{1}{s^2(s^2+1)} \student{= \dfrac{A}{s} + \dfrac{B}{s^2} +\dfrac{Cs+D}{s^2+1} }$}
\vfill
After partial fraction decomposition (try it for practice)\vfill
\algn{\student{A=0, B}&\student{=1, C=0, D=-1}\\
Y(s) &= \frac{1}{s^2}-\frac{1}{s^2+1}\\&=\lap{t} -\lap{\sin(t)}\\\\
y(t)&=t-\sin(t) 
}
}

\slide{Suppose we wish to solve \hfill  $\arr{rl}{ay\pp +by\p+cy&=g(t)\\y(0)&=0\\y\p(0)&=0}$ \hfill for general $g(t)$.\vfill
\student{\algn{as^2Y(s) + bsY(s)+cY(s)&=G(s)\\
Y(s)=\frac{G(s)}{as^2+bs+c} \\
Y(s)=\underbrace{F(s)G(s)}_{\text{How do we invert a product?}}&&\text{ with } F(s)=\frac{1}{as^2+bs+c}
}\vfill \centerline{We need to use the convolution theorem!}}
}

\subsection{Convolution Integrals}

\slide[Convolutions]{
We denote the convolution of two functions $f$ and $g$ by the symbol $f \ast g$, with \[h(t) =(f\ast g)(t) =\int_0^t f(\tau) g(t-\tau) d\tau\]
\textbf{Note:} $f \ast g = g\ast f$ (convolutions are symmetric)
\vfill
Convolutions are useful for inverting products of Laplace Transforms\\~\\

}
\slide{
\ex{Find $h(t)= t \ast t^2$}
\student{
\algn{h(t)&=\int_0^t (t-\tau) \tau^2 d\tau \\
&=\int_0^t t \tau^2 d\tau  - \int_{\tau=0}^t  \tau^3 d\tau\\
&= t \left[\frac{\tau^3}{3}\right]_{\tau=0^t} - \left[\frac{\tau^4}{4}\right]_0^t\\
&=\frac{t^4}{3} - \frac{t^4}{4}\\
&=\frac{t^4}{12} }
}
}

\slide{
\ex{Find $h(t)= t \ast \sin(t)$}
\student{
\algn{h(t)&=\int_0^t (t-\tau) \sin(\tau) d\tau \\
&=\int_0^t t \sin(\tau) d\tau  - \int_0^t  \tau \sin(\tau) d\tau & &\larray{\text{let}\\u=\tau, \quad du = d\tau\\ dv=\sin(\tau), v=-\cos(\tau)}\\
&= t \left[-\cos(\tau)\right]_{\tau=0}^t \\ &\phantom{=}- \left(-[\tau \cos(\tau)]_{\tau=0}^t + \int_0^t \cos(\tau) d\tau \right)\\
&=t -t\cos(t) - \paren{-t\cos(t) + \left[ \sin(\tau) \right]_{\tau=0}^t}\\
&=t-\sin(t) }
}
}

\subsection{Convolution Theorem}
\slide[Convolution Theorem]{\vspace{-.75em}
If $f(t)=\lapinv{F(s)}$ and $g(t)=\lapinv{G(s)}$ are known functions, then \vfill \[\boxed{ \lapinv{F(s) \cdot G(s)} =f \ast g } = \int _0^t f(\tau) g(t-\tau) d\tau =\int_0^t g(\tau)f(t-\tau)d\tau\]



\vfill
or conversely
\vfill
\[\boxed{\lap{f \ast g} = F(s) \cdot G(s)}\]
}
\slide[Proof of the convolution theorem]{\vspace{-2em}
\algn{\lap{h(t)} = \int_0^\infty e^{-st} h(t) dt = \int_{t=0}^\infty  \int _{\tau=0}^t f(\tau) g(t-\tau) e^{-st} d\tau\; dt}
\threemini[.32]{.3}{.3}{,3}{
\tikzplot{.1}{3}{.1}{1.75}{\tau}{t}{
\draw[domain=0:2 ] plot (\x,2*\x/3) node[right, yshift=-.1cm]{$t=\tau$};
\draw[pattern=horizontal lines, pattern color=\normcolor, thick] (0,0) -- (4,8/3) -- (0, 8/3);
}}{\[\carray{\text{equivalent areas}\\ \Leftrightarrow\\ \text{switch integration order}}\]}{
\tikzplot{.1}{3}{.1}{1.75}{\tau}{t}{
\draw[domain=0:2 ] plot (\x,2*\x/3) node[right, yshift=-.1cm]{$t=\tau$};
\draw[pattern=vertical lines, pattern color=\normcolor, thick] (0,0) -- (4,8/3) -- (0, 8/3);
}
}
\algn{&= \int_{\tau=0}^\infty  \int _{t=\tau}^\infty f(\tau) g(t-\tau) e^{-st} dt\; d\tau\\
&=\int_{\tau=0}^\infty f(\tau) e^{-s\tau} \int_{t=\tau}^\infty g(t-\tau) e^{-s(t-\tau)}d\tau\;dt &\text{let }u=t-\tau\\
&=\underbrace{\int_{\tau=0}^\infty f(\tau) e^{-s\tau} d\tau}_{F(s)} \underbrace{\int_{u=0}^\infty g(u) e^{-su} du}_{G(s)}  &t=\tau\Rightarrow u =0\\
&=F(s)G(s)}

}


\slide{Suppose $y(t)$ solves $y\pp+y=t,\quad y(0)=y\p(0)=0$. \vfill  Show that  $y(t)=\frac12 t^2 \ast \cos(t)$ and use the convolution theorem to find an explicit representation of y(t).\vfill

\twomini[.4]{.37}{.6}{
\student{\algn{s^2Y(s) + Y(s)  &= \frac{1}{s^2}\\
Y(s)&=\frac{1}{s^2\paren{s^2+1}}
}
}
}{
\student{\algn{\lap{\frac12 t^2 \ast \cos(t)} &= \frac12 \lap{t^2} \cdot \lap{\cos(t)}\\
&=\frac12 \frac{2}{s^3} \cdot \frac{s}{s^2+1}\\
&=\frac{1}{s^2\paren{s^2+1}} \checkmark
}
}

}

\student{
\algn{ Y(s) &= \frac{1}{s^2} \cdot \frac{1}{s^2+1}\\
&= \lap{t} \cdot \lap{\sin(t)}\\
y(t) &= t \ast \sin(t)=t-\sin(t)
}
}
}



\subsection{Solution Structure}
\slide[Inhomogeneous IVPs via Laplace transforms]{\vspace{-.75em}
Consider the constant coefficient 2$^{nd}$ order DE: $\arr{rl}{ay\pp +by\p+cy&=g(t)\\y(0)&=y_0\\y\p(0)&=v_0}$
Take LT\[ (as^2 + bs +c)Y(s)-(as+b)y_0-av_0 = G(s)\]
Solve for $Y(s)$:
\algn{Y(s)&=\student{\underbrace{\ucover{\frac{(as+b)y_0+av_0}{as^2 + bs +c} }}_{\carray{Y_h\\\scriptsize\text{effects of initial conditions}\\ \scriptsize\text{(Homogeneous Part)}}}} + \student{\underbrace{\ucover{\frac{G(s)}{as^2 + bs +c}}}_{\carray{Y_p\\\scriptsize\text{effects of forcing function}\\ \scriptsize\text{(Particular Part)}}}}
}
}



\slide[Inhomogeneous IVPs via Laplace transforms]{\vspace{-.75em}
 $\arr{rl}{ay\pp +by\p+cy&=g(t)\\y(0)&=y_0\\y\p(0)&=y\p_0}$\hfill$\rightarrow$\hfill
$Y(s)=\underbrace{\frac{(as+b)y_0+ay\p_0}{as^2 + bs +c} }_{Y_h(s)} + \underbrace{\frac{G(s)}{as^2 + bs +c}}_{Y_p(s)}$\vfill
\enum{\item Break up $Y_h(s)$ using partial frac. decomp. \& invert $Y_h(s) \rightarrow y_h(t)$.
\item Define the \alert{Transfer Function}: \[F(s)=\frac{1}{as^2+bs+c}\]
\item Invert $F(s) \rightarrow f(t)$. The function $f(t)$ is called the \alert{impulse response} function. 
\item From the convolution theorem with $Y_p(s)=F(s)G(s)$\[y_p(t) =f \ast g\]
\item Finally 
\[y(t)= y_h(t) + y_p(t)\]
}
}

\slide[]{
\ex{ $y\pp+4y=t^3,\quad y(0)=y\p(0)=0$.}
\vfill
Find an appropriate impulse response function and express the ODE's solution as a convolution integral.

\student{

\algn{\text{Transfer Function: }F(s)&=\frac{1}{s^2+4} = \frac12 \lap{\sin(2t)}\\
\text{Impulse Response: } f(t) &= \frac12 \sin(2t)\\\\
y(t) &= \sin(2t) \ast t^3\\& =\frac12 \int_0^t  \sin(2(t-\tau)) \tau^3 d\tau
}

}
}


\end{document}